Related: [[2.03 - Counting combinations]] [[2.07 - Probabilities using combinations]]

Look at the Venn diagram below for a finite sample space with two events.
$n(A ∩ B) = m$
$n(A) = p + m$
$n(B) = m + q$
It is obvious that $n(A ∪ B) = p + m + q$
so $n(A∪B) = p + m + m + q − m$
and $n(A ∪ B) = n(A) + n(B) − n(A ∩ B)$
Dividing by $n(S)$ gives $n\frac{A∪B}{n(S)}=n\frac{n(A)}{n(S)}+\frac{n(B)}{n(S)}-\frac{n(A ∩ B)}{n(S)}$
so $P(A-B) = P(A) + P(B) − P(A-and-B)$
![[Pasted image 20220608091422.png]]
The third probability rule means that this also applies to infinite sample spaces.