Related: [[3.04 - The sine rule]] [[3.03 - Area of a triangle]]
The cosine rule is a generalisation of Pythagoras’ theorem to cases where the triangle is not right angled.
![[Pasted image 20220607165918.png]]
In $\bigtriangleup ABC$, draw the perpendicular $AD$ with length $p$ and let $CD = x$.
Since $BC = a$, $BD = a – x$
From $ACD$
$b^{2}=x^{2}+p^{2}$
$\cos{C}=\frac{x}{b}$
$b\cos{C}=x$
From $\bigtriangleup DAB$
$c^{2}=p^{2}+(a-x)^{2}$
$=p^{2}+a^{2}-2ax+x^{2}$
$=p^{2}+x^{2}+a^{2}-2ax$
$c^{2}=b^{2}+a^{2}-2ax$
$c^{2}=b^{2}+a^{2}-2ax$
$c^{2}=b^{2}+a^{2}-2a(b\cos{C})$
$=a^{2}+b^{2}-2ab\cos{C}$
The cosine rule could also be written as
→ $a^{2}=b^{2}+c^{2}-2bc\cos{A}$
→ $b^{2}=a^{2}+c^{2}-2ac\cos{B}$
→ $c^{2}=b^{2}+a^{2}-2ab\cos{C}$
You can use the cosine rule to find an unknown side when given the other two sides and their included angle. The included angle is the angle formed by the two sides as shown below.
![[Pasted image 20220607170638.png]]
You can also use the cosine rule to find an unknown angle when given 3 sides. You can rearrange the cosine rule to make the formula easier to use.
$c^{2}=a^{2}+b^{2}-2ab\cos{C}$
$2ab\cos{C}=a^{2}+b^{2}-c^{2}$
$cos{C}=\frac{a^{2}+b^{2}-c^{2}}{2ab}$
The cosine rule could also be written as
→ $cos{A}=\frac{b^{2}+c^{2}-a^{2}}{2bc}$
→ $cos{B}=\frac{a^{2}+c^{2}-b^{2}}{2ac}$
→ $cos{C}=\frac{a^{2}+b^{2}-c^{2}}{2ab}$
Since $\cos{θ}$ is negative when $θ$ is obtuse, there are no ambiguous cases with the cosine rule.
You can use the cosine rule to help solve practical problems.