# Related
---
[[Radical and Fractional Indicies]]
[[Exponential Functions]]

# In-Class Lecture
---

>[!important]+ Index Laws
>$a^{m}\times a^{n}=a^{m+n}$
>$a^{m}\div a^{n}=a^{m-n}$
>$(a^{m})^{n}=a^{m\times n}$
>$(ab)^{n}=a^{n}b^{n}$
>$(\frac{a}{b})^{n}=\frac{a^{n}}{b^{n}}$
>$a^{0}=1$
>$a^{-n}=\frac{1}{a^{n}}$
>$\frac{1}{a^{-n}}=a^{n}$

>[!example]+
>$\frac{a^{-3}b^{2}}{c^{-1}}=\frac{c\times b^{2}}{a^{3}}=\frac{b^{2}c}{a^{3}}$

>[!example]+
>$\frac{1}{2^{1-n}}=2^{-(1-n)}=2^{n-1}$

>[!example]+ Simplify the following in positive-index form
>a) $12^{n}\times 18^{-2n}$
>	$=(2\times 3\times 2)^{n}\times (2\times 3\times 3)^{-2n}$
>	$=(2^{2}\times 3)^{n}\times (2\times 3^{2})^{-2n}$
>	$=2^{2n}\times 3^{n}\times 2^{-2n}\times 3^{-4n}$
>	$=2^{2n-2n}\times 3^{n-4n}$
>	$=1\times 3^{-3n}$
>	$=3^{-3n}$
>	$=\frac{1}{3^{3n}}$
>b) $\frac{3^{-3}\times 6^{4}\times 12^{-3}}{9^{-4}\times 2^{-2}}$
>	$=(3^{-3}\times 2^{4}\times 3^{4}\times 2^{-6}\times 3^{-3})/(3^{-4}\times 3^{-4}\times 2^{-2})$
>	$=\frac{3^{-2}\times 2^{-2}}{3^{-8}\times 2^{-2}}$
>	$=3^{6}$
>c) $\frac{3^{2n}\times 6^{n}}{8^{n}\times}3^{n}$
>	$=((3^{n}\times 3^{n})\times (3^{n}\times 2^{n}))/(2^{3n}\times 3^{n})$
>	$=\frac{3^{n}\times 3^{n}}{2^{2n}}$
>	$=(\frac{3}{2})^{2n}$


10)
	a) $\frac{x^{3}y^{5}}{xy^{2}}$ → $x^{2}y^{3}$
	b) $\frac{16a^{5}b\times 4a^{4}b^{3}}{8ab}$ → $8a^{8}b^{3}$
	c) $\frac{(-2xy)^{2}\times 2(x^{2}y)^{3}}{8(xy)^{3}}$ → $x^{5}y^{2}$
	d) $\frac{(-3x^{2}y^{3})^{2}}{(2xy)^{3}}\times \frac{4x^{4}y^{3}}{(xy)^{3}}$ → $\frac{9}{2}x^{2}y^{3}$
11)
	a) $m^{3}n^{2}p^{-2}\times (mn^{2}p)^{-3}$ → $\frac{1}{n^{4}p^{5}}$
	b) $\frac{x^{3}yz^{-2}\times 2(x^{3}y^{-2}z)^{2}}{xyz^{-1}}$ → $\frac{2x^{8}z}{y^{4}}$
	c) $\frac{a^{2}b\times (ab^{-2})^{-3}}{(a^{-2}b_{-1})^{-2}}$ → $\frac{b^{5}}{a^{5}}$
	d) $\frac{a^{2}b^{3}c^{-4}}{a^{-1}b^{2}c^{-3}}$ → $\frac{a^{3}b}{c}$
	e) $\frac{a^{2n-1}\times b^{3}\times c^{1-n}}{a^{n-3}\times b^{2-n}\times c^{2-2n}}$ → $a^{n+2}b^{n+1}c^{n-1}$
12)
	a) $3^{4n}\times 9^{2n}\times 27^{3n}$ → $3^{17n}$
	b) $\frac{2^{n}\times 8^{n+1}}{32^{n}}$ → $2^{3-n}$
	c) $\frac{3^{n-1}\times 9^{2n-3}}{6^{2}\times 3^{n+2}}$ → $\frac{3^{4n-11}}{2^{2}}$
	d) $\frac{2^{2n}\times 9^{2n-1}}{6^{n-1}}$ → $2^{n+1}3^{3n-1}$
	e) $\frac{25^{2n}\times 5^{n-1}}{5^{2n+1}}$ → $5^{3n-2}$
	f) $\frac{6^{x-3}\times 4^{x}}{3^{x+1}}$ → $2^{3x-3}\times 3^{-4}$
	g) $\frac{6^{2n}\times 9^{3}}{27^{n}\times 8^{n}\times 16^{n}}$ → $3^{6-n}\times 2^{-5n}$
	h) $\frac{3^{n-2}\times 9^{n+1}}{27^{n-1}}$ → $3^{3}=27$
	i) $\frac{8\times 2^{5}\times 3^{7}}{9\times 2^{7}\times 81}$ → $6$

# Textbook 11.01 (pg 494)
---
You have previously seen that the term $a^{n}$ is called a power where:
	$a^{n}=a\times a\times a\times ...\times a$ (to $n$ factors)
For the power, $a^{n}$, $n$ is called the index or exponent and $a$ is called the base.
There are some general laws that simplify calculations with indicies.
Each of the index laws can be proved from first principles using the definition:
$a^{n}=a\times a\times a\times ...$ (to $n$ factors)
>[!important]+ Index Laws
>$a^{m}\times a^{n}=a^{m+n}$
>$a^{m}\div a^{n}=a^{m-n}$
>$(a^{m})^{n}=a^{mn}$
>$(ab)^{n}=a^{n}b^{n}$
>$(\frac{a}{b})^{n}=\frac{a^{n}}{b^{n}}$

>[!example]+ Example 1
>Prove that $(ab)^{n}=a^{n}b^{n}$
>$(ab)^{n}=ab\times ab\times ab\times ...$ (to $n$ factors)
>$=(a\times a\times a\times ...)\times (b\times b\times b\times ...)$
>$=a^{n}\times a^{n}$
>$a^{n}b^{n}$

>[!example]+ Example 2
>Simplify
>a) $m^{9}\times m^{7}\div m^{2}$
>	$=m^{9+7-2}$
>	$m^{14}$
>b) $(sy^{4})^{3}$
>	$=2^{3}\times y^{4\times 3}$
>	$8y^{12}$

You can extend the definition of powers to cover the index of zero and negative indicies.

>[!important]
>$a^{0}=1 (a\neq 0)$
>$a^{-n}=\frac{1}{a^{n}} (a\neq 0)$

>[!example]+ Example 3
>Simplifty and express with positive indicies:
>a) $\frac{4h^{-6}\times 3h^{2}}{h^{-3}\times 6h^{5}}$
>	$=\frac{12}{6}\times h^-6+2-(-3)-5$
>	$2h^{-6}$
>	$\frac{2}{h^{6}}$
>b) $\frac{2^{m-n}\times 3^{m-n}\times 6^{n}}{12^{m}}$
>	$=\frac{2^{m-n}\times 3^{m-n}\times (2\times 3)^{n}}{(2^{2}\times 3)^{m}}$
>	$=\frac{2^{m-n}\times 3^{m-n}\times 2^{n}\times 3^{n}}{2^{2m}\times 3^{m}}$
>	$=2^{m-n+n-2n}\times 3^{m-n+n-m}$
>	$=2^{-m}\times 3^{0}$
>	$=\frac{1}{2^{m}}\times 1$
>	$=\frac{1}{2^{m}}$



# Ex 11.01
---
5)
	a) $(pq^{3})^{5}$ → $p^{5}q^{15}$
	b) $(\frac{a}{b})^{8}$ → $\frac{a^{8}}{b^{8}}$
	c) $(\frac{4a}{b^{4}})^{3}$ → $\frac{4a^{8}}{b^{12}}$
	d) $7(a^{3}b)^{2}$ → $7a^{6}b^{2}$
	e) $\frac{(2m^{7})^{3}}{m^{4}}$ → $\frac{2m^{11}}{m^{4}}$
	f) $(\frac{xy^{3}\times(xy^{2})^{4}}{xy}$ → $x^{4}y^{10}$
	g) $\frac{(2k^{8})^{4}}{(6k^{3})^{3}}$ → $2k^{32}/6k^{9}$
	h) $(2y^{5})^{7}\times\frac{y^{12}}{8}$ → $16y^{47}$
	i) $(\frac{a^{6}\times a^{4}}{a^{11}})^{-3}$ → $a^{3}$
	j) $(\frac{5xy^{9}}{x^{8}\times y^{3}})^{3}$ → $125x^{-21}y^{18}$
6)
	a) $r^{-6}\times r^{4}$ → $\frac{1}{r^{2}}$
	b) $4y^{-5}\times3y^{-4}$ → $\frac{12}{y^{9}}$
	c) $\frac{12p^{6}\times6p^{-2}}{8p^{-1}\times3p}$ → $\frac{64a^{3}}{b^{12}}$
	d) $\frac{4j^{5}\times5j^{-4}}{10j^{7}}$ → $7a^{6}b^{2}$
	e) $\frac{2m^{3}\times m^{-10}}{12m^{6}}$ → $8m^{17}$
	f) $\frac{5k^{-3}}{2k^{4}}\div\frac{10k^{5}}{k^{-2}}$ → $\frac{1}{4k^{14}}$
	g) $3g^{-3}h^{4}\times5g^{4}h^{-6}$ → $\frac{15g}{h^{2}}$
	h) $5k^{3}m^{-6}\times (k^{-3}m^{-4})^{-5}$ → $5k^{18}m^{14}$
	i) $\frac{8v^{-4}w^{2}\times 4v^{10}w^{-8}}{2vw^{-9}\times v^{-6}w^{3}}$ → $16v^{11}$
	j) $\frac{12p^{-4}q^{-3}\times (2pq^{4})^{2}}{(3p^{-1}q^{4})^{-3}}$ → $\frac{4q^{17}}{p^{13}}$
	k) $((\frac{e^{2}f^{4}}{e^{-5}f})^{3})\times\frac{4e^{-3}f^{4}}{3e^{6}f^{6}}$ → $\frac{4e^{12}f^{7}}{3}$
	l) $\frac{c^{7}d^{8}}{d^{-5}}\div \frac{(8c^{-2}d^{3})^{2}}{4^{-2}c^{-2}d^{3}}$ → $\frac{c^{9}d^{10}}{1024}$
7) $2^{3}(\frac{3}{4})^{2}$ → $\frac{9}{2}$
8) $\frac{x^{3}y^{2}}{xy^{5}}$ → $324$
9) $\frac{a^{2}b^{3}}{c^{4}}$ → $\frac{64}{27}$
10) $\frac{a^{11}b^{8}}{a^{8}b^{7}}$ → $\frac{1}{25}$
11) $\frac{p^{5}q^{8}r^{4}}{p^{4}q^{6}r^{2}}$ → $\frac{7}{32}$