# Related
---
[[Index Laws]]
# In-Class Lecture
---
Radical Indicies
>[!important]+ Rules of indicies
>$a^{\frac{1}{2}}\times a^{\frac{1}{2}}=a^{\frac{1}{2}+\frac{1}{2}}=a^{1}=a$
>$\sqrt{a}\times\sqrt{a}=a$
>$a^\frac{1}{n}=\sqrt[n]{a}$
>$\sqrt[n]{a^{m}}$
>	$=(a^{m})^{\frac{1}{n}}$
>	$=a^{\frac{m}{n}}$
>$a^{\frac{m}{n}}=\sqrt[n]{a^{m}}$

>[!example]+ Write as a single power of 2:
>a) $\sqrt[3]{2}$
>	$=2^{\frac{1}{3}}$
>b) $\frac{1}{\sqrt{2}}$
>	$=\frac{1}{2^{\frac{1}{2}}}$
>	$=2^{-\frac{1}{2}}$
>c) $\sqrt[5]{4}$
>	$=(2^{2})^{\frac{1}{5}}$
>	$=2^{2\times \frac{1}{5}}$
>	$=2^{\frac{2}{5}}$

>[!example]+ Without using a calculator, write in the simplest rational form:
>a) $8^{\frac{4}{3}}$
>	$=(2^{3})^\frac{4}{3}$
>	$=2^{3\times \frac{4}{3}}$
>	$=2^{4}$
>	$=16$
>b) $27^{-\frac{2}{3}}$
>	$=(3^{3})^-\frac{2}{3}$
>	$3^{3\times-\frac{2}{3}}$
>	$3^{-2}$
>	$\frac{1}{9}$

>[!example]+ Simplifty:
>a) $\frac{3^\frac{1}{4}\times\sqrt{6}\times\sqrt[4]{2}}{16^{\frac{3}{4}}}$
>	$=\frac{3^{\frac{1}{4}}\times3^{\frac{1}{2}}\times2^{\frac{1}{2}}\times2^{\frac{1}{4}}}{(16^{\frac{1}{4}})^{3}}$
>	$=\frac{3^{\frac{1}{4}}\times3^{\frac{1}{2}}\times2^{\frac{1}{2}}\times2^{\frac{1}{4}}}{2^{3}}$
>	$=\frac{3^{\frac{3}{4}}\times2^{\frac{3}{4}}}{2^{3}}$
>	$=\frac{3^{\frac{3}{4}}}{2^{\frac{12}{4}-\frac{3}{4}}}$
>	$=\frac{3^{\frac{3}{4}}}{2^{\frac{9}{4}}}$
>b) $(x^{-2}y)^{\frac{1}{2}}\times(\frac{x}{y^{-3}})^{4}$
>	$=x^{-1}y^{\frac{1}{2}}\times\frac{x^{4}}{y^{-12}}$
>	$=x^{3}\times y^{\frac{25}{2}}$

>[!example]+ Simplify:
>2)
>	a) $\sqrt[3]{a^{2}b}\div\sqrt{ab^{3}}$ → $a^{\frac{1}{6}}b^{-\frac{7}{6}}$
>	b) $(a^{-2}b)^{3}\times(\frac{1}{b^{-3}})^{\frac{1}{2}}$ →$a^{-6}b^{\frac{9}{2}}$
>	c) $\frac{45^{\frac{1}{3}}}{9^{\frac{3}{4}}\times15^{\frac{3}{2}}}$ → $3^{-\frac{7}{3}}\times5^{-\frac{7}{6}}$
>	d) $2^{\frac{3}{2}}\times4^{-\frac{1}{4}}\times16^{-\frac{3}{4}}$ → $\frac{1}{4}$
>	e) $(\frac{x^{3}y^{-2}}{x^{4}y^{-2}})^{-2}\div(\frac{3^{-3}x^{-2}y}{x^{4}y^{-2}})^{2}$ → $x^{6}y^{-8}$
>	f) $(\sqrt[5]{a^{2}})^\frac{3}{2}\times(\sqrt[3]{a^{5}})^{\frac{1}{5}}$ → $a^{\frac{14}{15}}$
>3)
>	a) $(2x-1)\sqrt{2x-1}$ → $(2x-1)^{\frac{3}{2}}$
>	b) $(x-1)^{2}\sqrt{x-1}$ → $(x-1)^{\frac{5}{2}}$
>	c) $(x^{2}+1)\sqrt{x^{2}+1}$ → $(x^{2}+1)^{\frac{3}{2}}$
>	d) $(x-1)^{3}\sqrt{x-1}$ → $(x-1)^{\frac{7}{2}}$
>	e) $\frac{1}{\sqrt{x-1}}+\sqrt{x-1}$ → $x(x-1)^{-\frac{1}{2}}$
>	f) $(5x^{2}+1)\sqrt[3]{5x^{2}+1}$ → $(5x^{2}+1)^{\frac{4}{3}}$

# Textbook 11.02 (pg 498)
---
It is possible for indicies to be fractional
Suppose that $a^{\frac{1}{9}}$ exists. Then you can do the following:
	$(a^{\frac{1}{q}})^{q}=a^{(\frac{1}{q}\times q})=a^{1}=a$
So, $a^{\frac{1}{q}}$ to the power of $q$ would be $a$. In other words, for the laws to be consistent, $a^{\frac{1}{q}}$ would have to be the $q$th root of $a$. This means that:
$a^{\frac{1}{9}}=\sqrt[q]{a}$
and $a^{\frac{p}{q}}=(a^{p})^{\frac{1}{9}}$ or $(a^{\frac{1}{9}})^{p}$ so $a^{\frac{p}{q}}=\sqrt[q]{(a)^{p}}=(\sqrt[q]{a})^{p}$
Now the square root of a negative number is not real, and neither is any even root of a negative number. For example, there are no real numbers for $\sqrt{-4}$ or $\sqrt[4]{-81}$.

>[!important]+ Index laws for rational indices.
>$a^{\frac{1}{9}}=\sqrt[q]{a}$
>$a^{-\frac{1}{q}}=\frac{1}{\sqrt[q]{a}}$
>$a^{\frac{p}{q}}=\sqrt[q]{(a)^{p}}=(\sqrt[q]{a})^{p}$

This means that the procedure for $a^{\frac{p}{q}}$ will not always work in cases where $a$ is negative. As well as that, the concept of a $q$th root only makes sense if $q$ is positive. For this reason it is assumed that q is positive for fractional indices. If $q$ is negative, then the fractional power has to be rewritten so that the qth root part is positive.
The square root sign, $\sqrt{}$, is also called the radical sign, and numbers such as $\sqrt{7}$ and $\sqrt[3]{12}$ are known as radicals.
The definitions of powers can be extended to rational indices.

# Ex 11.02
---
 3)
	 a) $k^{\frac{1}{2}}$
	 b) $3^{\frac{1}{4}}$
	 c) $5^{\frac{1}{2}}$
	 d) $4^{\frac{1}{5}}$
	 e) $w^{\frac{1}{3}}$
	 f) $c^{\frac{3}{2}}$
	 g) $64^{\frac{4}{3}}$
	 h) $e^{\frac{3}{4}}$
	 i) $28^{\frac{4}{9}}$
	 j) $q^{\frac{6}{5}}$
	 k) $8^{\frac{1}{5}}$
	 l) $16^{\frac{7}{6}}$
 4)
	 a) $t^{\frac{1}{2}}$
	 b) $y^{\frac{1}{5}}$
	 c) $x^{\frac{3}{2}}$
	 d) $(9-x)^{\frac{1}{3}}$
	 e) $(4s+1)^{\frac{1}{2}}$
	 f) $(2t+3)^{-\frac{1}{2}}$
	 g) $(5x-y)^{-\frac{3}{2}}$
	 h) $(3x+1)^{\frac{5}{2}}$
	 i) $(x-2)^{-\frac{2}{3}}$
	 j) $\frac{1}{2}(y+7)^{-\frac{1}{2}}$
	 k) $5(x+4)^{-\frac{1}{3}}$
	 l) $\frac{3}{5}(x^{2}+2)^{-\frac{3}{4}}$
 5)
	 a) $a^{4\frac{1}{2}}$
	 b) $b^{3 \frac{1}{2}}$
	 c) $\frac{6}{n^{\frac{1}{2}}}$
	 d) $12g^{6\frac{1}{3}}$
	 e) $12w^{3 \frac{2}{3}}p^{2 \frac{1}{2}}$
	 f) $10m^{3\frac{1}{2}}n^{2\frac{1}{3}}$
	 g) $\frac{21u^{3}}{s^{3\frac{1}{2}}}$
	 h) $\frac{24p^{1\frac{1}{2}}}{q^{\frac{5}{12}}}$
 6)
	 a) $x+x^{2}+2x^{\frac{3}{2}}$
	 b) $a^{\frac{2}{3}}-b^{\frac{2}{3}}$
	 c) $p^{2}+p^{-1}+2p^{\frac{1}{2}}$
	 d) $x+x-1+2$
	 e) $x^{-\frac{1}{2}}$
 7)
	 a) $\frac{1}{\sqrt[3]{a-2b}}$
	 b) $\frac{1}{\sqrt[3]{(y-3)^{2}}}$
	 c) $\frac{4}{\sqrt[7]{(6a+1)^{4}}}$
	 d) $\frac{1}{3\sqrt[5]{(x+y)^{4}}}$
	 e) $\frac{6}{7\sqrt[9]{(3x+8)^{2}}}$